Lem.dfy
@@ -4,32 +4,21 @@ module Lem {
   import opened Type
   import opened Property
 
-  function makeRootBlack(t: Rb_tree): Rb_tree
-  {
-    match t
-    case Node(_, k, l, r) => Node(Black, k, l, r)
-    case Null => Null
-  }
-
-  lemma lem_make_black (t:Rb_tree)
-    ensures root_property2(makeRootBlack(t)) {
-  }
-
   lemma bst_meaning(t:Rb_tree)
-    requires t.Node? &&t.left.Node? && t.right.Node? && bst_property(t)
-    ensures t.left.key < t.key
-    ensures t.right.key > t.key
+    requires t.Node? && bst_property(t)
+    ensures !t.left.Node? || t.left.key < t.key
+    ensures !t.right.Node? || t.right.key > t.key
   {
-    assert t.left.key in contain(t.left);
+    // assert t.left.key in contain(t.left);
     assert forall x :: x in contain(t.left) ==> x < t.key;
-    assert t.left.key < t.key;
+    //assert t.left.key < t.key;
 
-    assert t.right.key in contain(t.right);
+    //assert t.right.key in contain(t.right);
     assert forall x :: x in contain(t.right) ==> x > t.key;
-    assert t.right.key > t.key;
+    // assert t.right.key > t.key;
   }
   lemma bst_transitivity_right(t:Rb_tree)
-    requires t.Node? &&t.left.Node? && t.right.Node? && bst_property(t)
+    requires t.Node? &&t.left.Node? && bst_property(t)
     ensures forall x :: x in contain (t.left.right)==> x < t.key
 
   {
@@ -39,4 +28,19 @@ module Lem {
     assert forall x :: x in contain(t.left.right) ==> x in contain(t.left);
 
   }
+
+  lemma bst_transitivity_left(t:Rb_tree)
+    requires t.Node? && t.right.Node? && bst_property(t)
+    ensures forall x :: x in contain (t.right.left)==> x > t.key
+
+  {
+    assert bst_property(t);
+    assert bst_property(t.right);
+    assert bst_property(t.left);
+    assert forall x :: x in contain(t.right.left) ==> x in contain(t.right);
+  }
+
+  lemma blackHeight_lem(t:Rb_tree)
+    ensures BlackHeight2(t) != -1 ==> BlackHeight2(t) > 0
+  {}
 }
