Operations.dfy
@@ -15,18 +15,32 @@ module Operations {
     case _ => false
   }
 
-  function rotate_left(h: Rb_tree) : Rb_tree
+  method rotate_left(h: Rb_tree) returns (result: Rb_tree)
     requires right_leaning_red_link(h)
-    ensures !right_leaning_red_link(rotate_left(h))
+    requires bst_property(h)
+    requires black_property2(h)
+    ensures !right_leaning_red_link(result)
+    ensures bst_property(result)
+    ensures contain(h) == contain(result)
+    ensures result.color == h.color
+    ensures result.left.Node? && result.left.color == Red
+    ensures isRed(result.left)
+    ensures black_property2(result)
+    ensures BlackHeight2(h) == BlackHeight2(result)
+
     decreases h
   {
-    match h
-    case Node(h_color, h_key, h_left, h_right) =>
-      match h_right
-      case Node(Red, x_key, x_left, x_right) =>
-        var new_h := Node(Red, h_key, h_left, x_left);
-        var new_x := Node(h_color, x_key, new_h, x_right);
-        new_x
+    var new_h := Node(Red, h.key, h.left, h.right.left);
+    result := Node(h.color, h.right.key, new_h, h.right.right);
+    bst_meaning(h);
+    bst_transitivity_left(h);
+    assert bst_property(result.left);
+    assert bst_property(result.right);
+    assert result.left.Node?;
+    assert BlackHeight2(h.left) == BlackHeight2(h.right);
+    assert h.right.color == Red;
+    assert BlackHeight2(h.right) == BlackHeight2(h.right.left);
+    return;
   }
 
 
@@ -40,12 +54,16 @@ module Operations {
 
   method rotate_right(h: Rb_tree) returns (result: Rb_tree)
     requires double_left_red_link(h)
-    requires h.Node?
-    requires h.right.Node?
-    requires double_left_red_link(h)
+    requires black_property2(h)
     requires bst_property(h)
     ensures bst_property(result)
     ensures contain(result) == contain(h)
+    ensures BlackHeight2(result) == BlackHeight2(h)
+    ensures black_property2(result)
+    ensures result.color == h.color
+    ensures isRed(result.left)
+    ensures isRed(result.right)
+    ensures BlackHeight2(h) == BlackHeight2(result)
     decreases h
   {
     var new_h := Node(Red, h.key, h.left.right, h.right);
@@ -77,18 +95,20 @@ module Operations {
   {
     match h
     // I think we might need to help dafny to prove that this node is black
-    case Node(Black, _, Node(Red, _, _, _), Node(Red, _, _, _)) => true
+    case Node(_, _, Node(Red, _, _, _), Node(Red, _, _, _)) => true
     case _ => false
   }
-
 
 
   method flip_color(h: Rb_tree) returns (result : Rb_tree)
     requires hasRedChildren(h)
     requires bst_property(h)
+    requires black_property2(h)
     ensures bst_property(result)
     ensures equal_content_property(result, h)
     ensures !hasRedChildren(result)
+    ensures BlackHeight2(h) == BlackHeight2(result)
+    ensures black_property2(result)
     decreases h
   {
     var new_left := Node(Black, h.left.key, h.left.left, h.left.right);
@@ -99,14 +119,26 @@ module Operations {
     assert contain(new_left) == contain(h.left);
     assert contain(new_right) == contain(h.right);
     assert contain(result) == contain(new_left) + contain(new_right) + {h.key};
+
+    assert h.left.color == Red && h.right.color == Red;
+    assert h.color == Black;
+    assert BlackHeight2(h) == BlackHeight2(h.left) + 1;
+    assert BlackHeight2(new_left) == BlackHeight2(h.left) + 1;
+    assert BlackHeight2(new_right) == BlackHeight2(h.right) + 1;
+    assert BlackHeight2(result) == BlackHeight2(new_left);
+    assert BlackHeight2(new_left) != -1;
     return;
   }
 
   method insert_recur(t: Rb_tree, insert_key: int) returns (result :Rb_tree)
     decreases t
     requires bst_property(t)
+    requires black_property2(t)
+    requires llrb_property(t)
     ensures bst_property(result)
     ensures contain(result) == contain(t) + {insert_key}
+    ensures black_property2(result)
+    ensures BlackHeight2(result) == BlackHeight2(t)
 
   {
     if t.Null? {
@@ -122,32 +154,85 @@ module Operations {
         assert contain(r) == {insert_key} + contain(t.right);
         assert forall x :: x in contain(r) ==> x > t.key;
         assert bst_property(result);
+        assert black_property2(r);
+        assert BlackHeight2(r) == BlackHeight2(t.right);
       } else if insert_key < t.key {
         var l := insert_recur(t.left, insert_key);
+        assert (black_property2(l));
         result := Node(t.color, t.key, l, t.right);
         assert forall x :: x in contain(t.right) ==> x > insert_key;
       } else {
         result := t;
+        assert black_property2(result);
       }
+
+      // We need to assert several properties before the rebalance to satisfy post-condition
+      // assert red_property2(result.left); this cannot be proved rn
+      // assert red_property2(result.right);this cannot be proved rn
+      assert black_property2(result);
+      assert BlackHeight2(result) == BlackHeight2(t);
+
+      if hasRedChildren(result) {
+        result := flip_color(result);
+      }
+
+      if right_leaning_red_link(result) {
+        assert result.Node?;
+        assert result.right.Node? && result.right.color == Red;
+        assert result.left.Null? || result.left.color == Black;
+        result := rotate_left(result);
+      }
+
+      if double_left_red_link(result) {
+        result := rotate_right(result);
+      }
+
+
     }
     return;
 
+  }
+
+  method makeRootBlack(t: Rb_tree) returns(result: Rb_tree)
+    requires bst_property(t)
+    requires black_property2(t)
+    requires !t.Node? || red_property2(t.left)
+    requires !t.Node? || red_property2(t.right)
+
+    ensures bst_property(result)
+    ensures root_property2(result)
+    ensures black_property2(result)
+    ensures contain(t) == contain(result)
+  {
+    blackHeight_lem(t);
+    if t.Node? {
+      assert BlackHeight2(t) != -1;
+      assert BlackHeight2(t.left) != -1;
+      // We want to tell dafny that we are greater than 0
+
+      result := Node(Black, t.key, t.left, t.right);
+      assert BlackHeight2(result) == 1 + BlackHeight2(t.left);
+    }
+    else {
+      result := Null;
+      assert BlackHeight2(result) == 1;
+    }
+    return;
   }
 
   // Wrapper function for the recursive and then change root color
   method insert(t: Rb_tree, key: int) returns (root:Rb_tree)
     requires root_property2(t)
     requires bst_property(t)
-    // requires red_property2(t)
-    // requires black_property2(t)
-    // requires left_leaning_property(t)
+    requires red_property2(t)
+    requires black_property2(t)
     ensures root_property2(root)
     ensures bst_property(root)
     ensures contain(root) == contain(t) + {key}
+    ensures black_property2(root)
   {
     root := insert_recur(t, key);
     root := makeRootBlack(root);
-    lem_make_black(root);
     return;
   }
 }
